GCounter constructor

src/gcounter.lean
@@ -2,92 +2,120 @@ import tactic
 
 def gcounter (n: ℕ) : Type := array n ℕ
 
+def new (n: ℕ) : gcounter n := { data := λ _, 0 }
+
 def inc {n: ℕ} (g: gcounter n) (index: fin n) (value: ℕ) : gcounter n :=
-  g.write index $ g.read index + value
+	g.write index $ g.read index + value
 
 def merge {n: ℕ} (g₁: gcounter n) (g₂: gcounter n) : gcounter n :=
-  array.map₂ max g₁ g₂
+	array.map₂ max g₁ g₂
 
 def value {n: ℕ} (g: gcounter n) : ℕ :=
-  array.foldl g 0 (+)
+	array.foldl g 0 (+)
 
 lemma merge_idempotent {n: ℕ} (g: gcounter n) : merge g g = g :=
 begin
-  dsimp only [merge],
-  apply array.ext,
-  intro,
-  simp only [array.read_map₂, max_eq_right, eq_self_iff_true],
+	dsimp only [merge],
+	apply array.ext,
+	intro,
+	simp only [array.read_map₂, max_eq_right, eq_self_iff_true],
 end
 
 lemma merge_commutative {n: ℕ} (g₁ g₂: gcounter n) : merge g₁ g₂ = merge g₂ g₁ :=
 begin
-  dsimp only [merge],
-  apply array.ext,
-  intro,
-  simp only [array.read_map₂, max_comm],
+	dsimp only [merge],
+	apply array.ext,
+	intro,
+	simp only [array.read_map₂, max_comm],
 end
 
 lemma merge_associative
  {n: ℕ} (g₁ g₂ g₃: gcounter n) : merge g₁ (merge g₂ g₃) = merge (merge g₁ g₂) g₃ :=
 begin
-  dsimp only [merge],
-  apply array.ext,
-  intro,
-  simp only [array.read_map₂, max_assoc],
+	dsimp only [merge],
+	apply array.ext,
+	intro,
+	simp only [array.read_map₂, max_assoc],
 end
 
 lemma inc_merge_increasing
-  {n: ℕ} (v: ℕ) (i: fin n) (g: gcounter n) : merge (inc g i v) g = inc g i v :=
+	{n: ℕ} (v: ℕ) (i: fin n) (g: gcounter n) : merge (inc g i v) g = inc g i v :=
 begin
-  dsimp only [merge, inc],
-  apply array.ext,
-  intro,
-  simp only [array.read_map₂, max_eq_left_iff],
+	dsimp only [merge, inc],
+	apply array.ext,
+	intro,
+	simp only [array.read_map₂, max_eq_left_iff],
 
-  by_cases i = i_1,
-  simp only [h, array.read_write],
-  linarith,
+	by_cases i = i_1,
+	simp only [h, array.read_write],
+	linarith,
 
-  rwa array.read_write_of_ne,
+	rwa array.read_write_of_ne,
 end
 
 lemma inc_value_increasing_aux₁
-  (a b: ℕ) (li: list ℕ) : list.foldl (+) (a + b) li = list.foldl (+) a li + b :=
+	(a b: ℕ) (li: list ℕ) : list.foldl (+) (a + b) li = list.foldl (+) a li + b :=
 begin
-  induction li generalizing a b,
-  refl,
-  simp only [list.foldl, add_right_comm, li_ih],
+	induction li generalizing a b,
+	refl,
+	simp only [list.foldl, add_right_comm, li_ih],
 end
 
 lemma inc_value_increasing_aux₂
-  (a b i_val: ℕ) (li: list ℕ) (h: i_val < li.length):
-  list.foldl has_add.add a (li.update_nth i_val (li.nth_le i_val h + b)) =
-  list.foldl has_add.add a li + b :=
+	(a b i_val: ℕ) (li: list ℕ) (h: i_val < li.length):
+	list.foldl has_add.add a (li.update_nth i_val (li.nth_le i_val h + b)) =
+	list.foldl has_add.add a li + b :=
 begin
-  induction li generalizing a b i_val,
-  
-  rw list.length at h,
-  linarith,
-  
-  cases i_val,
-  simp only [list.update_nth, list.nth_le, list.foldl, ← add_assoc],
+	induction li generalizing a b i_val,
+	
+	rw list.length at h,
+	linarith,
+	
+	cases i_val,
+	simp only [list.update_nth, list.nth_le, list.foldl, ← add_assoc],
 
-  apply inc_value_increasing_aux₁,
-  apply li_ih,
+	apply inc_value_increasing_aux₁,
+	apply li_ih,
 end
 
 lemma inc_value_increasing
-  {n: ℕ} (v: ℕ) (i: fin n) (g: gcounter n) : value (inc g i v) = value g + v :=
+	{n: ℕ} (v: ℕ) (i: fin n) (g: gcounter n) : value (inc g i v) = value g + v :=
 begin
-  simp only [inc, value, ← array.to_list_foldl, array.write_to_list],
+	simp only [inc, value, ← array.to_list_foldl, array.write_to_list],
 
-  cases i,
-  rw [← array.to_list_nth_le],
+	cases i,
+	rw [← array.to_list_nth_le],
 
-  generalize h : array.to_list g = li,
-  simp only [h, add_comm],
-  rw [add_comm, add_comm v],
-  apply inc_value_increasing_aux₂,
-  
-  rwa array.to_list_length,
+	generalize h : array.to_list g = li,
+	simp only [h, add_comm],
+	rw [add_comm, add_comm v],
+	apply inc_value_increasing_aux₂,
+	
+	rwa array.to_list_length,
+end
+
+lemma value_new_aux₁ {n: ℕ} : (new n).to_list = list.repeat 0 n :=
+begin
+	apply list.ext_le,
+	simp only [array.to_list_length, list.length_repeat],
+
+	intros,
+	rw [list.nth_le_repeat],
+	rw [list.length_repeat] at h₂,
+
+	rw array.to_list_nth_le,
+	simp only [new, array.read, d_array.read],
+	assumption,
+end
+
+lemma value_new_aux₂ {n: ℕ} : list.foldl (+) 0 (list.repeat 0 n) = 0 :=
+begin
+	induction n,
+	simp only [list.repeat, list.foldl, add_zero],
+	assumption,
+end
+
+lemma value_new {n: ℕ} : value (new n) = 0 :=
+begin
+	simp only [value, ← array.to_list_foldl, add_comm, value_new_aux₁, value_new_aux₂],
 end
